README.md
@@ -1,5 +1,17 @@
-# Mines Nancy — Parcours Recherche
+# Mines Nancy — Research Project — _Vincent Trélat_
+
+> ## Introduction
+>
+> This repository was created as part of my research project at Mines de Nancy, supervised by [Stephan Merz](https://members.loria.fr/Stephan.Merz/). The objective of the project is to mechanize a proof of correctness of a set-based algorithm inspired by Tarjan's algorithm for computing the strongly connected components of a graph. The algorithm is detailed in [Vincent Bloemen's thesis](https://ris.utwente.nl/ws/portalfiles/portal/122499728/thesis.pdf) and a few invariants are described.
+
 ---
-* This git repository contains my personal implementation of Tarjan's algorithm for the strongly connected components problem.
-* The algorithm is implemented in __Java__, see ```Graph.java``` for the actual SCC algorithm and compile/execute ```Main.java```.
-* Graphs are represented through the adjency list of each node, _i.e._ if nodes are numbered from _0_ to _n-1_, then for _i_ in _[0, n-1]_, `adjency[i]` is the list of nodes to which node i is connected.
+
+> ## Formal methods
+>
+> The formal proof is written is [Isabelle(HOL)](https://isabelle.in.tum.de). I also wrote a LaTeX paper [on the proof](/LaTeX/report.pdf).
+
+---
+
+> ## Model Checking
+>
+> A TLA+ model for checking our invariants is provided in [here](/tla).
